check

DenotSem/Deterministic.thy
@@ -4,68 +4,7 @@ begin
 
 lemma wf_eval: "\<lbrakk> v \<in> \<lbrakk>e\<rbrakk>\<rho>; wf_env \<rho> \<rbrakk> \<Longrightarrow> wf_ty v"
   apply (induction e) apply (case_tac "x < length \<rho>") apply force+ done
-
-lemma merge_inter: "A ~ B \<Longrightarrow> merge A B \<approx> A \<sqinter> B"
-  apply (case_tac A)
-    apply (case_tac B)
-      apply force
-    apply force
-  apply force
-  apply force
-  apply force
-  done
     
-lemma merge_inter_equiv: "\<lbrakk> A ~ B; B \<approx> B' \<rbrakk> \<Longrightarrow> merge A B \<approx> A \<sqinter> B'"
-  apply (case_tac A)
-    apply (case_tac B)
-      apply force
-     apply force
-    apply force
-   apply force
-    apply force
-  done
-  
-lemma fold_merge_equiv_fold_meet_aux: fixes xs::"ty list"
-  assumes c_xs: "\<forall>v1 v2. {v1,v2} \<subseteq> set xs \<longrightarrow> v1 ~ v2" and x_xp: "x \<approx> x'" and
-    x_xs: "\<forall>v. v \<in> set xs \<longrightarrow> x ~ v" and wf_xs: "\<forall>v. v \<in> set xs \<longrightarrow> wf_ty v" and wf_x: "wf_ty x" 
-  shows "fold merge xs x \<approx> fold op \<sqinter> xs x'"
-  using c_xs x_xp x_xs wf_xs wf_x
-proof (induction xs arbitrary: x x')
-  case Nil
-  then show ?case by auto
-next
-  case (Cons a xs)
-  have 1: "\<forall>v1 v2. {v1, v2} \<subseteq> set xs \<longrightarrow> v1 ~ v2" using Cons by auto
-  have 2: "\<forall>v. v \<in> set xs \<longrightarrow> (merge a x) ~ v" using Cons apply clarify 
-      apply (rule consis_merge_left) apply auto done
-  have 3: "\<forall>v. v \<in> set xs \<longrightarrow> wf_ty v" using Cons by auto
-  have 4: "wf_ty (merge a x)" using Cons wf_merge consis_sym by auto
-  have 5: "merge a x \<approx> a \<sqinter> x'"
-  proof -
-    have "a ~ x" using Cons(4) consis_sym by auto
-    then show ?thesis using Cons(3) merge_inter_equiv[of a x x'] by simp
-  qed
-  have "fold merge xs (merge a x) \<approx> fold op \<sqinter> xs (a \<sqinter> x')"
-    using Cons.IH[of "merge a x" "a \<sqinter> x'"] 1 2 3 4 5 by blast  
-  then show ?case by simp
-qed
-
-lemma merge_list_equiv_meet_list: fixes xs::"ty list"
-  assumes c_xs: "\<forall>v1 v2. {v1,v2} \<subseteq> set xs \<longrightarrow> v1 ~ v2" and wf_xs: "\<forall>v. v \<in> set xs \<longrightarrow> wf_ty v" 
-    and xs_ne: "xs \<noteq> []"
-  shows "\<Prod>xs \<approx> \<Sqinter>xs"
-proof -
-  obtain x xs' where xs: "xs = x#xs'" using xs_ne by (cases xs) auto      
-  have 1: "\<forall>v1 v2. {v1,v2} \<subseteq> set xs' \<longrightarrow> v1 ~ v2" using c_xs xs by auto
-  have 2: "x \<approx> x" by auto
-  have 3: "\<forall>v. v \<in> set xs' \<longrightarrow> x ~ v" using c_xs xs by auto
-  have 4: "\<forall>v. v \<in> set xs' \<longrightarrow> wf_ty v" using wf_xs xs by auto
-  have 5: "wf_ty x" using wf_xs xs by auto
-  have "fold merge xs' x \<approx> fold op \<sqinter> xs' x" 
-    using 1 2 3 4 5 fold_merge_equiv_fold_meet_aux[of xs' x x] by blast
-  then show ?thesis using xs merge_list_def meet_list_def by simp
-qed
-  
 lemma consis_codomain:
   fixes a b c d
   assumes ab_g1: "a\<rightarrow>b \<in> set \<Gamma>1" and cd_g2: "c\<rightarrow>d \<in> set \<Gamma>2" and
@@ -83,10 +22,11 @@ proof -
     show "b ~ d" using ab_cd a_c by simp 
 qed
 
-lemma all_fun_ex: "\<lbrakk> all_funs \<Gamma>; x \<in> set \<Gamma>; \<And> a b. \<lbrakk> x = a \<rightarrow> b \<rbrakk> \<Longrightarrow> P \<rbrakk> \<Longrightarrow> P"
+    
+lemma all_fun_ex: "\<lbrakk> all_funs (set \<Gamma>); x \<in> set \<Gamma>; \<And> a b. \<lbrakk> x = a \<rightarrow> b \<rbrakk> \<Longrightarrow> P \<rbrakk> \<Longrightarrow> P"
   apply (cases x) apply auto done
 
-lemma all_fun_ex_dom: "\<lbrakk> all_funs \<Gamma>; y \<in> set (map cod \<Gamma>) \<rbrakk> \<Longrightarrow> \<exists>x. x\<rightarrow>y \<in> set \<Gamma>"
+lemma all_fun_ex_dom: "\<lbrakk> all_funs (set \<Gamma>); y \<in> set (map cod \<Gamma>) \<rbrakk> \<Longrightarrow> \<exists>x. x\<rightarrow>y \<in> set \<Gamma>"
   apply (induction \<Gamma> arbitrary: y)
   apply force
   apply simp apply (erule disjE) 
@@ -102,11 +42,11 @@ proof -
   have f1_v11: "f1 <: v1 \<rightarrow> v1'" using f1_v1 by simp
   have f2_v22: "f2 <: v2 \<rightarrow> v2'" using f2_v2 by simp
       
-  obtain \<Gamma>1 where g1_ne: "\<Gamma>1 \<noteq> []" and af_g1: "all_funs \<Gamma>1" and g1_f1: "set \<Gamma>1 \<subseteq> atoms f1" and
+  obtain \<Gamma>1 where g1_ne: "\<Gamma>1 \<noteq> []" and af_g1: "all_funs (set \<Gamma>1)" and g1_f1: "set \<Gamma>1 \<subseteq> atoms f1" and
     v1_g1: "\<forall>v v'. v\<rightarrow>v' \<in> set \<Gamma>1 \<longrightarrow> v1 <: v" and g1_v1p: "\<Sqinter>(map cod \<Gamma>1) <: v1'"
     using f1_v11 sub_fun_any_inv_atoms[of f1 v1 v1'] by blast
   let ?C1 = "map cod \<Gamma>1"     
-  obtain \<Gamma>2 where g2_ne: "\<Gamma>2 \<noteq> []" and af_g2: "all_funs \<Gamma>2" and g2_f2: "set \<Gamma>2 \<subseteq> atoms f2" and
+  obtain \<Gamma>2 where g2_ne: "\<Gamma>2 \<noteq> []" and af_g2: "all_funs (set \<Gamma>2)" and g2_f2: "set \<Gamma>2 \<subseteq> atoms f2" and
     v2_g2: "\<forall>v v'. v\<rightarrow>v' \<in> set \<Gamma>2 \<longrightarrow> v2 <: v" and g2_v2p: "\<Sqinter>(map cod \<Gamma>2) <: v2'"
     using f2_v22 sub_fun_any_inv_atoms[of f2 v2 v2'] by blast
   let ?C2 = "map cod \<Gamma>2"
@@ -139,8 +79,12 @@ proof -
       apply (rule consis_codomain[of d1 v1' \<Gamma>2 d2 v2' \<Gamma>2 v2 v2 f2 f2])
       using v11_g2 v22_g2 v2_g2 consis_refl wf_v2 wf_f2 g2_f2 by auto   
   qed
-  have c1_c2: "\<Prod>?C1 ~ \<Prod>?C2"
-  proof (rule consis_merge_list)
+  have c1_c2: "\<Sqinter>?C1 ~ \<Sqinter>?C2" 
+  proof (rule meet_list_consis)
+    show "map cod \<Gamma>1 \<noteq> []" using g1_ne by auto
+  next
+    show "map cod \<Gamma>2 \<noteq> []" using g2_ne by auto
+  next
     show "\<forall>v1 v2. {v1, v2} \<subseteq> set ?C1 \<union> set ?C2 \<longrightarrow> v1 ~ v2"
     proof clarify
       fix v1' v2' assume 1: "{v1',v2'} \<subseteq> set ?C1 \<union> set ?C2"        
@@ -170,37 +114,314 @@ proof -
         have "v1' ~ v2'" using v1_c2 v2_c2 c_c2 g2_ne by auto 
       } ultimately show "v1' ~ v2'" using 1 by blast
     qed      
-  next
-    show "\<forall>v. v \<in> set ?C1 \<longrightarrow> wf_ty v" using wf_c1 by blast
-  next
-    show "\<forall>v. v \<in> set ?C2 \<longrightarrow> wf_ty v" using wf_c2 by blast
-  next
-    show "map cod \<Gamma>1 \<noteq> []" using g1_ne by simp
-  next
-    show "map cod \<Gamma>2 \<noteq> []" using g2_ne by simp
-  qed
-  have c1_c1: "\<Prod>?C1 \<approx> \<Sqinter>?C1" using merge_list_equiv_meet_list wf_c1 c_c1 g1_ne by auto
-  have c2_c2: "\<Prod>?C2 \<approx> \<Sqinter>?C2" using merge_list_equiv_meet_list wf_c2 c_c2 g2_ne by auto    
-  have "\<Sqinter>?C1 ~ \<Sqinter>?C2" using c1_c1 c1_c2 c2_c2 
-      using consis_le ty_equiv_def by auto 
+  qed  
   then show ?thesis using g1_v1p g2_v2p consis_le by blast
 qed
-  
-lemma merge_app: assumes f1_v1: "v1' \<in> f1 \<bullet> v1" and f2_v2: "v2' \<in> f2 \<bullet> v2" and 
+
+lemma inter_app: assumes f1_v1: "v1' \<in> f1 \<bullet> v1" and f2_v2: "v2' \<in> f2 \<bullet> v2" and 
   f1_f2: "f1 ~ f2" and v1_v2: "v1 ~ v2" and v1p_v2p: "v1' ~ v2'"
-  shows "merge v1' v2' \<in> merge f1 f2 \<bullet> merge v1 v2"
+  shows "v1' \<sqinter> v2' \<in> (f1 \<sqinter> f2) \<bullet> (v1 \<sqinter> v2)"
 proof -
-  have wf_v12: "wf_ty (merge v1' v2')" using f1_v1 f2_v2 v1p_v2p by auto 
+  have wf_v12: "wf_ty (v1' \<sqinter> v2')" using f1_v1 f2_v2 v1p_v2p by auto 
   have f1_v1p: "f1 <: v1 \<rightarrow> v1'" using f1_v1 by simp
   have f2_v2p: "f2 <: v2 \<rightarrow> v2'" using f2_v2 by simp  
-  have "merge f1 f2 <: f1 \<sqinter> f2" using merge_inter f1_f2 ty_equiv_def by auto
-  also have "f1 \<sqinter> f2 <: (v1\<rightarrow>v1') \<sqinter> (v2\<rightarrow>v2')" using f1_v1p f2_v2p by (rule sub_mon)
+  have "f1 \<sqinter> f2 <: (v1\<rightarrow>v1') \<sqinter> (v2\<rightarrow>v2')" using f1_v1p f2_v2p by (rule sub_mon)
   also have "(v1 \<rightarrow> v1') \<sqinter> (v2 \<rightarrow> v2') <: (v1 \<sqinter> v2) \<rightarrow> (v1' \<sqinter> v2')" by (rule sub_dist_union_fun)
-  also have "... <: (merge v1 v2) \<rightarrow> (merge v1' v2')" apply (rule sub_arrow)
-      using merge_inter v1_v2 v1p_v2p ty_equiv_def apply auto done
-  finally have "merge f1 f2 <: (merge v1 v2) \<rightarrow> (merge v1' v2')" using sub_trans by auto
+  finally have "f1 \<sqinter> f2 <: (v1 \<sqinter> v2) \<rightarrow> (v1' \<sqinter> v2')" using sub_trans by auto
   then show ?thesis using wf_v12 by simp
 qed
+
+lemma weaken_env_fun: "\<lbrakk> F v e \<rho>1; \<rho>2 <: \<rho>1; (\<forall> v \<rho>1 \<rho>2. v \<in> \<lbrakk>e\<rbrakk>\<rho>1 \<longrightarrow> \<rho>2 <: \<rho>1 \<longrightarrow> v \<in> \<lbrakk>e\<rbrakk>\<rho>2) \<rbrakk>
+                    \<Longrightarrow> F v e \<rho>2"
+proof (induction v arbitrary: e \<rho>1 \<rho>2)
+  case (TNat n)
+  then have "False" by auto
+  then show ?case ..
+next
+  case (TArrow v1 v2)
+  have "v1#\<rho>2 <: v1#\<rho>1" using TArrow.prems(2) apply auto apply (case_tac k) apply auto done
+  then show ?case using TArrow by simp
+next
+  case (TInter v1 v2)
+  then show ?case by auto    
+qed    
+  
+lemma weaken_env: "\<lbrakk> v \<in> \<lbrakk>e\<rbrakk>\<rho>1; \<rho>2 <: \<rho>1 \<rbrakk> \<Longrightarrow> v \<in> \<lbrakk>e\<rbrakk>\<rho>2"
+proof  (induction e arbitrary: v \<rho>1 \<rho>2)
+  case (EVar x)
+  then show ?case 
+    apply (case_tac "x < length \<rho>1") using sub_trans apply force apply force done
+next
+  case (ENat n)
+  then show ?case by auto
+next
+  case (ELam e)
+  then show ?case using weaken_env_fun[of v e \<rho>1 \<rho>2] by auto
+next
+  case (EApp e1 e2)
+  then show ?case apply simp apply blast done      
+next
+  case (EPrim x1a e1 e2)
+  then show ?case apply simp apply blast done
+next
+  case (EIf e1 e2 e3)
+  then show ?case apply simp apply blast done
+qed
+
+lemma denot_fun_atoms: "\<lbrakk> all_funs (atoms v); \<forall>v1 v2. v1\<rightarrow>v2 \<in> atoms v \<longrightarrow> v2 \<in> \<lbrakk>e\<rbrakk>v1#\<rho> \<rbrakk>
+   \<Longrightarrow> F v e \<rho>"
+  by (induction v) auto    
+
+lemma denot_fun_inv_atoms: "F v e \<rho> \<Longrightarrow> all_funs (atoms v) 
+   \<and> (\<forall>v1 v2. v1\<rightarrow>v2 \<in> atoms v \<longrightarrow> v2 \<in> \<lbrakk>e\<rbrakk>v1#\<rho>)"
+  apply (induction v) apply auto done
+    
+lemma eval_fun_all_funs: "F v e \<rho> \<Longrightarrow> all_funs (atoms v)"
+  apply (induction v) apply auto done
+
+abbreviation subsump :: "ty \<Rightarrow> ty \<Rightarrow> exp \<Rightarrow> ty list \<Rightarrow> bool" where
+  "subsump v1 v2 e \<rho> \<equiv> v1 \<in> \<lbrakk>e\<rbrakk>\<rho> \<longrightarrow> v1 <: v2 \<longrightarrow> wf_ty v2 \<longrightarrow> wf_env \<rho> \<longrightarrow> v2 \<in> \<lbrakk>e\<rbrakk>\<rho>" 
+
+abbreviation determ :: "ty \<Rightarrow> ty \<Rightarrow> exp \<Rightarrow> ty list \<Rightarrow> ty list \<Rightarrow> bool" where
+  "determ v1 v2 e \<rho>1 \<rho>2 \<equiv> v1\<in> \<lbrakk>e\<rbrakk>\<rho>1 \<longrightarrow> v2\<in> \<lbrakk>e\<rbrakk>\<rho>2 \<longrightarrow> wf_env \<rho>1 \<longrightarrow> wf_env \<rho>2 \<longrightarrow> consis_env \<rho>1 \<rho>2
+    \<longrightarrow> v1 \<sqinter> v2 \<in> \<lbrakk>e\<rbrakk>(\<rho>1\<sqinter>\<rho>2) \<and> wf_ty (v1 \<sqinter> v2)"
+
+lemma fun_eval_distr_determ:
+  "\<lbrakk> F (A \<rightarrow> B \<sqinter> C \<rightarrow> D) e \<rho>; \<forall>v1 v2 \<rho>1 \<rho>2. determ v1 v2 e \<rho>1 \<rho>2; wf_env \<rho>; wf_ty A; wf_ty C; A ~ C \<rbrakk>
+    \<Longrightarrow> F ((A \<sqinter> C) \<rightarrow> (B \<sqinter> D)) e \<rho>"
+  apply simp apply clarify
+  apply (subgoal_tac "(A\<sqinter>C)#\<rho> <: A # \<rho>") prefer 2 apply simp 
+   apply clarify apply (case_tac k) apply force apply force
+  apply (subgoal_tac "(A\<sqinter>C)#\<rho> <: C # \<rho>") prefer 2 apply simp 
+   apply clarify apply (case_tac k) apply force apply force
+  apply (subgoal_tac "B \<in> \<lbrakk>e\<rbrakk>(A\<sqinter>C)#\<rho>") prefer 2 using weaken_env apply blast
+  apply (subgoal_tac "D \<in> \<lbrakk>e\<rbrakk>(A\<sqinter>C)#\<rho>") prefer 2 using weaken_env apply blast
+  apply (subgoal_tac "wf_env ((A\<sqinter>C)#\<rho>)") prefer 2 apply simp apply clarify
+    apply (case_tac k) apply simp apply blast apply force
+  apply (subgoal_tac "B \<sqinter> D \<in> \<lbrakk>e\<rbrakk>((A \<sqinter> C) # \<rho>) \<sqinter> ((A \<sqinter> C) # \<rho>)") prefer 2 apply blast
+  apply (subgoal_tac "(A \<sqinter> C) # \<rho> <: ((A \<sqinter> C) # \<rho>) \<sqinter> ((A \<sqinter> C) # \<rho>)") prefer 2
+   apply simp apply clarify apply (case_tac k) prefer 2 apply force
+    apply simp 
+  apply blast
+  apply (rule weaken_env)    
+   apply blast
+    apply blast
+  done
+ 
+lemma denot_fold_meet_inv_init: "F (fold op \<sqinter> L A) e \<rho> \<Longrightarrow> F A e \<rho>"
+  apply (induction L arbitrary: A)
+   apply force
+  apply simp
+  apply (subgoal_tac "F (a \<sqinter> A) e \<rho>") prefer 2 apply blast
+  apply simp
+  done    
+
+lemma denot_fold_meet_swap_init: "\<lbrakk> F (fold op \<sqinter> L A) e \<rho>; F B e \<rho> \<rbrakk> 
+   \<Longrightarrow>  F (fold op \<sqinter> L B) e \<rho>"
+  apply (induction L arbitrary: A B) apply force
+  apply simp 
+  apply (subgoal_tac "F (a \<sqinter> A) e \<rho>") prefer 2 using denot_fold_meet_inv_init apply blast
+  apply (subgoal_tac "F (a \<sqinter> B) e \<rho>") prefer 2 apply force
+  apply blast  
+  done    
+
+abbreviation consis_funs :: "ty list \<Rightarrow> bool" where
+  "consis_funs L \<equiv> \<forall>v1 v1' v2 v2'. {v1\<rightarrow>v1',v2\<rightarrow>v2'} \<subseteq> (set L) \<longrightarrow> v1 ~ v2 \<and> v1' ~ v2'"  
+
+abbreviation wf_list :: "ty list \<Rightarrow> bool" where
+  "wf_list L \<equiv> \<forall>v. v \<in> set L \<longrightarrow> wf_ty v"
+ 
+lemma denot_fun_fold_meet:
+  "\<lbrakk> F (fold op \<sqinter> L (A\<rightarrow>B)) e \<rho>; all_funs (set L); wf_env \<rho>; wf_ty A; wf_ty B;
+     wf_list L; consis_funs ((A\<rightarrow>B)#L);
+     \<forall>v1 v2 \<rho>1 \<rho>2. determ v1 v2 e \<rho>1 \<rho>2 \<rbrakk> \<Longrightarrow> 
+    F ((fold op \<sqinter> (map dom L) A) \<rightarrow> (fold op \<sqinter> (map cod L) B)) e \<rho>"
+  apply (induction L arbitrary: A B)
+   apply force
+   apply (case_tac a) apply force defer apply force
+  apply (rename_tac A' B') apply clarify    
+  apply (subgoal_tac "F (fold op \<sqinter> L ((A'\<sqinter>A) \<rightarrow> (B' \<sqinter> B))) e \<rho>") prefer 2
+   apply (rule denot_fold_meet_swap_init)
+    apply force
+   apply (rule fun_eval_distr_determ)
+   apply (subgoal_tac "F (A' \<rightarrow> B' \<sqinter> A \<rightarrow> B) e \<rho>") prefer 2
+         apply (rule denot_fold_meet_inv_init)
+         apply force
+   apply assumption apply assumption apply assumption 
+   apply force
+    apply assumption
+  apply (metis bot_least consis_sym insert_mono list.set(2))
+  apply (subgoal_tac "wf_ty (A'\<sqinter>A)") 
+   apply (subgoal_tac "wf_ty (B'\<sqinter>B)")
+   apply (subgoal_tac "\<forall>v1 v1' v2 v2'. {v1\<rightarrow>v1',v2\<rightarrow>v2'} \<subseteq> insert ((A'\<sqinter>A)\<rightarrow>(B'\<sqinter>B)) (set L) \<longrightarrow> v1 ~ v2 \<and> v1' ~ v2'")
+     apply simp
+    defer
+      
+    apply (subgoal_tac "B ~ B'") prefer 2 
+     apply (metis bot_least insert_mono list.set(2))
+    apply (subgoal_tac "wf_ty B'") prefer 2 apply auto[1]
+    apply (subgoal_tac "B' ~ B") prefer 2 apply (rule consis_sym) apply blast
+    apply blast
+    
+    apply (subgoal_tac "A ~ A'") prefer 2 
+      apply (metis bot_least insert_mono list.set(2))
+    apply (subgoal_tac "wf_ty A'") prefer 2 apply auto[1]
+    apply (subgoal_tac "A' ~ A") prefer 2 apply (rule consis_sym) apply blast
+   apply blast
+    apply clarify
+proof -
+  fix a L A B A' B' v1 v1' v2 v2'
+  assume 1: "consis_funs ((A \<rightarrow> B) # (A' \<rightarrow> B') # L)"
+    and 2: "{v1 \<rightarrow> v1', v2 \<rightarrow> v2'} \<subseteq> insert ((A' \<sqinter> A) \<rightarrow> (B' \<sqinter> B)) (set L)"
+    and "wf_ty A'" and "wf_ty A" and "wf_ty B" and "wf_ty B'" and "A' ~ A" and "B'~B"    
+  have "v1 \<rightarrow> v1' = (A'\<sqinter>A)\<rightarrow>(B'\<sqinter>B) \<or> v1\<rightarrow>v1' \<in> set L" using 2 apply auto done
+  then show "v1 ~ v2 \<and> v1' ~ v2' "
+  proof 
+    assume v11: "v1 \<rightarrow> v1' = (A'\<sqinter>A)\<rightarrow>(B'\<sqinter>B)"
+    have "v2 \<rightarrow> v2' = (A'\<sqinter>A)\<rightarrow>(B'\<sqinter>B) \<or> v2\<rightarrow>v2' \<in> set L" using 2 apply auto done
+    then show "v1 ~ v2 \<and> v1' ~ v2' "
+    proof
+      assume v22: "v2 \<rightarrow> v2' = (A'\<sqinter>A)\<rightarrow>(B'\<sqinter>B)"
+      show ?thesis using v22 v11 apply simp 
+        by (simp add: \<open>A' ~ A\<close> \<open>B' ~ B\<close> \<open>wf_ty A'\<close> \<open>wf_ty A\<close> \<open>wf_ty B'\<close> \<open>wf_ty B\<close> 
+            consis_refl consis_sym)
+    next
+      assume v22: "v2 \<rightarrow> v2' \<in> set L"
+      have ap_v2: "A' ~ v2" using 1 v22 apply auto done
+      have a_v2: "A ~ v2" using 1 v22 apply auto done
+      have aa_v2: "A'\<sqinter>A ~ v2" using ap_v2 a_v2 apply blast done
+      have bp_v2p: "B' ~ v2'" using 1 v22 apply auto done
+      have b_v2: "B ~ v2'" using 1 v22 apply auto done
+      have bb_v2: "B'\<sqinter>B ~ v2'" using bp_v2p b_v2 apply blast done          
+      show ?thesis using v11 v22 aa_v2 bb_v2 apply simp done
+    qed
+  next
+    assume v11: "v1 \<rightarrow> v1' \<in> set L"
+    have "v2 \<rightarrow> v2' = (A'\<sqinter>A)\<rightarrow>(B'\<sqinter>B) \<or> v2\<rightarrow>v2' \<in> set L" using 2 apply auto done
+    then show "v1 ~ v2 \<and> v1' ~ v2' "
+    proof
+      assume v22: "v2 \<rightarrow> v2' = (A'\<sqinter>A)\<rightarrow>(B'\<sqinter>B)"
+      have ap_v1: "A' ~ v1" using 1 v22 v11 apply auto done
+      have a_v1: "A ~ v1" using 1 v22 v11 apply auto done
+      have aa_v1: "A'\<sqinter>A ~ v1" using ap_v1 a_v1 apply blast done
+          
+      have bp_v2p: "B' ~ v1'" using 1 v22 v11 apply auto done
+      have b_v2: "B ~ v1'" using 1 v22 v11 apply auto done
+      have bb_v2: "B'\<sqinter>B ~ v1'" using bp_v2p b_v2 apply blast done          
+
+      show ?thesis using v11 v22 aa_v1 bb_v2 consis_sym apply simp done
+    next
+      assume v22: "v2 \<rightarrow> v2' \<in> set L"
+      show ?thesis using v11 v22 1 apply auto done
+    qed 
+  qed    
+qed
+  
+lemma denot_fun_meet_list: "\<lbrakk> F (\<Sqinter>L) e \<rho>; L \<noteq> []; all_funs (set L); wf_env \<rho>;
+   consis_funs L; wf_list L;
+   \<forall> v1 v2 \<rho>1 \<rho>2. determ v1 v2 e \<rho>1 \<rho>2 \<rbrakk> 
+  \<Longrightarrow> F (\<Sqinter>(map dom L) \<rightarrow> \<Sqinter>(map cod L)) e \<rho>"
+  apply (cases L) apply force
+  unfolding meet_list_def apply clarify
+  apply (case_tac a) apply force defer apply force apply simp
+  apply (subgoal_tac "wf_ty x21") prefer 2 apply blast
+  apply (subgoal_tac "wf_ty x22") prefer 2 apply blast    
+    using denot_fun_fold_meet apply simp 
+  done
+    
+lemma subsumption_fun: fixes v1::ty and v2::ty
+  assumes v1_e: "F v1 e \<rho>" and v1_v2: "v1 <: v2" and
+    wf_v1: "wf_ty v1"  and wf_v2: "wf_ty v2" and wf_r: "wf_env \<rho>" and
+    IH: "\<forall>v1 v2 \<rho>. subsump v1 v2 e \<rho>" and
+    D: "\<forall> v1 v2 \<rho>1 \<rho>2. determ v1 v2 e \<rho>1 \<rho>2"
+  shows "F v2 e \<rho>"
+proof (rule denot_fun_atoms)
+  have "all_funs (atoms v1)" using v1_e eval_fun_all_funs by simp
+  then show "all_funs (atoms v2)" using v1_v2 
+    using d_fun_atoms_L_inv sub_ty_def by auto 
+next
+  show "\<forall>v1 v2a. v1 \<rightarrow> v2a \<in> atoms v2 \<longrightarrow> v2a \<in> \<lbrakk>e\<rbrakk>v1 # \<rho>"
+  proof clarify
+    fix A B assume ab_v2: "A \<rightarrow> B \<in> atoms v2"
+    have v1_ab: "v1 <: A \<rightarrow> B" using v1_v2 ab_v2 sub_atom_sub by blast
+    then show "B \<in> \<lbrakk>e\<rbrakk>A#\<rho>"
+    proof (rule sub_any_fun_elim)
+      fix \<Gamma>1 assume g_ne: "\<Gamma>1 \<noteq> []" and af_g: "all_funs (set \<Gamma>1)" and 
+        gp_v1: "set \<Gamma>1 \<subseteq> atoms v1" and
+        a_g1: "\<forall>v v'. v \<rightarrow> v' \<in> set \<Gamma>1 \<longrightarrow> A <: v" and
+        cg_b: "\<Sqinter> (map cod \<Gamma>1) <: B"
+      have a_dg: "A <: \<Sqinter> (map dom \<Gamma>1)" using a_g1 meet_list_ub af_g g_ne by blast
+      have wf_B: "wf_ty B" using wf_v2 ab_v2 wf_ty_arrow_inv by blast
+      have af_v1: "all_funs (atoms v1)" and 
+        v1_e_atoms: "\<forall>v v'. v\<rightarrow>v' \<in> atoms v1 \<longrightarrow> v' \<in> \<lbrakk>e\<rbrakk>v#\<rho>"
+        using v1_e denot_fun_inv_atoms[of v1 e \<rho>] by auto
+      have c_g1: "consis_funs \<Gamma>1"
+        apply clarify apply (rename_tac W X Y Z)
+        apply (subgoal_tac "W\<rightarrow>X \<in> atoms v1") prefer 2 using gp_v1 af_g apply auto[1] 
+        apply (subgoal_tac "Y\<rightarrow>Z \<in> atoms v1") prefer 2 using gp_v1 af_g apply auto[1] 
+        by (metis wf_v1 a_g1 ab_v2 consis_le consis_refl consistent.simps(4) insert_subset 
+            wf_atoms wf_consis_atoms wf_ty_arrow_inv wf_v2)        
+      have wf_g1: "wf_list \<Gamma>1" using gp_v1 wf_v1 by blast
+      have ag1: "atoms (\<Sqinter>\<Gamma>1) = ctx_atoms \<Gamma>1" 
+        by (simp add: g_ne)
+      have af_mg1: "all_funs (atoms (\<Sqinter>\<Gamma>1))" using af_g ag1 apply auto
+          apply (case_tac x) apply auto done
+      have "atoms (\<Sqinter>\<Gamma>1) \<subseteq> atoms v1" using ag1 gp_v1 af_g apply simp
+        apply (rule subsetI) apply simp apply clarify 
+        apply (case_tac xa) apply auto done
+      then have "F (\<Sqinter>\<Gamma>1) e \<rho>" using v1_e_atoms af_mg1 denot_fun_atoms by blast
+      then have "F (\<Sqinter>(map dom \<Gamma>1) \<rightarrow> \<Sqinter>(map cod \<Gamma>1)) e \<rho>"
+        using denot_fun_meet_list D af_g g_ne wf_r c_g1 wf_g1 by blast
+      then have cg1_e: "\<Sqinter> (map cod \<Gamma>1) \<in> \<lbrakk>e\<rbrakk>(\<Sqinter> (map dom \<Gamma>1))#\<rho>" by simp
+      have "A#\<rho> <: (\<Sqinter> (map dom \<Gamma>1))#\<rho>" using a_dg apply auto apply (case_tac k) apply auto done
+      then have cg1_e: "\<Sqinter> (map cod \<Gamma>1) \<in> \<lbrakk>e\<rbrakk>A#\<rho>" using cg1_e weaken_env by blast
+      have "wf_ty A" using wf_v2 ab_v2 wf_ty_arrow_inv by blast
+      then have "wf_env (A#\<rho>)" using wf_r apply auto apply (case_tac k) apply auto done
+      then show ?thesis using cg1_e IH cg_b wf_B by blast
+    qed
+  qed
+qed
+  
+lemma subsumption_deterministic:
+  "(\<forall> v1 v2 \<rho>. subsump v1 v2 e \<rho>) \<and> (\<forall> v1 v2 \<rho>1 \<rho>2. determ v1 v2 e \<rho>1 \<rho>2)"
+proof (induction)
+  case (EVar x)
+  show ?case
+  proof
+    show "\<forall>v1 v2 \<rho>. subsump v1 v2 (EVar x) \<rho>" apply clarify
+      apply (case_tac "x < length \<rho>") defer apply force
+      apply simp apply (rule sub_trans) apply auto done
+  next
+    show "\<forall>v1 v2 \<rho>1 \<rho>2. determ v1 v2 (EVar x) \<rho>1 \<rho>2" apply clarify
+      apply (case_tac "x < length \<rho>1") defer apply force
+      using consis_le inter_func by auto
+  qed
+next
+  case (ENat n)
+  then show ?case apply auto
+    using sub_trans apply blast
+    by (simp add: consis_le inter_func)      
+next
+  case (ELam e)
+  show ?case
+  proof
+    show "\<forall>v1 v2 \<rho>. subsump v1 v2 (\<lambda> e) \<rho>" 
+      apply clarify apply simp
+       apply (rule subsumption_fun) apply blast apply blast apply blast 
+         apply blast apply blast using ELam.IH apply auto done
+  next
+    show "\<forall>v1 v2 \<rho>1 \<rho>2. determ v1 v2 (\<lambda> e) \<rho>1 \<rho>2 " sorry
+  qed
+next
+  case (EApp e1 e2)
+  then show ?case sorry
+next
+  case (EPrim x1a e1 e2)
+  then show ?case sorry
+next
+  case (EIf e1 e2 e3)
+  then show ?case sorry
+qed  
 
 (*
 lemma strengthen_env: "\<lbrakk> v1 \<in> \<lbrakk>e\<rbrakk>\<rho>1; \<rho>2 <: \<rho>1; wf_env \<rho>1; wf_env \<rho>2 \<rbrakk> \<Longrightarrow>
@@ -384,7 +605,7 @@ next
   have v1p_v2p: "v1' ~ v2'"
     using f1_f2 v1_v2 v1p_f1_v1 v2p_f2_v2 wf_f1 wf_f2 wf_v1 wf_v2 consistent_app by blast
   have m_v12p_f12_v12: "merge v1' v2' \<in> (merge f1 f2) \<bullet> (merge v1 v2)"
-    using v1p_f1_v1 v2p_f2_v2 f1_f2 v1_v2 v1p_v2p merge_app by blast
+    using v1p_f1_v1 v2p_f2_v2 f1_f2 v1_v2 v1p_v2p inter_app by blast
   show ?case using v1p_v2p m_v12p_f12_v12 m_f1f2 m_v12 by auto
 next
   case (EPrim f e1 e2)
@@ -429,7 +650,7 @@ next
   qed    
 qed
 *)
-  
+(*
 abbreviation strengthen :: "ty \<Rightarrow> ty \<Rightarrow> exp \<Rightarrow> ty list \<Rightarrow> ty list \<Rightarrow> bool" where
   "strengthen v1 v2 e \<rho>1 \<rho>2 \<equiv> (v1 \<in> \<lbrakk>e\<rbrakk>\<rho>1 \<and> \<rho>2 <: \<rho>1 \<and> v1 <: v2
                                \<and> wf_ty v2 \<and> wf_env \<rho>1 \<and> wf_env \<rho>2
@@ -813,5 +1034,6 @@ next
      by (smt Cons.prems(4) aa_bb_le insert_subset list.simps(15))     
   then show ?case using a by simp
 qed
-    
+*)
+  
 end
