DenotSem/Consistency.thy
@@ -133,203 +133,12 @@ lemma atoms_consis: "\<forall> v1' v2'. v1' \<in> atoms v1 \<longrightarrow> v2'
 
 lemma atoms_inconsis: "\<lbrakk> \<not>(v1' ~ v2'); v1' \<in> atoms v1; v2' \<in> atoms v2 \<rbrakk> \<Longrightarrow> \<not>(v1 ~ v2)"
   by (induction v1 v2 arbitrary: v1' v2' rule: consistent.induct) auto
-
-(*
-lemma consis_merge: "\<lbrakk> a ~ b; a ~ y; x ~ b; x ~ y \<rbrakk> \<Longrightarrow> merge a x ~ merge b y"
-  apply (case_tac a) apply (case_tac b) apply auto apply (case_tac y) apply auto
-    apply (case_tac x) apply auto apply (case_tac b) apply auto apply (case_tac b)
-    apply auto
-  done
-*)
   
 lemma consis_inter_L[intro!]: "\<lbrakk> v1 ~ v3; v2 ~ v3 \<rbrakk> \<Longrightarrow> v1 \<sqinter> v2 ~ v3"
   using atoms_consis consis_atoms by blast
     
 lemma consis_inter_R[intro!]: "\<lbrakk> v1 ~ v2; v1 ~ v3 \<rbrakk> \<Longrightarrow> v1 ~ v2 \<sqinter> v3"
   using atoms_consis consis_atoms by blast
-    
-(*
-lemma consis_merge_left: "\<lbrakk> a ~ v; x ~ v; wf_ty a; wf_ty x \<rbrakk> \<Longrightarrow> merge a x ~ v"
-  apply (case_tac a) apply (case_tac v) apply auto apply (case_tac x) apply auto
-   apply (case_tac v) apply auto apply (case_tac x) apply auto 
-    apply (rule consis_inter_right) apply blast apply blast apply blast apply blast
-   apply (case_tac x) apply force apply force apply simp 
-   apply clarify apply (rule consis_inter_right) apply blast apply blast apply blast apply blast
-  apply (case_tac v) apply force apply force apply simp
-  apply (case_tac x) apply force apply simp apply clarify apply (rule conjI)
-    apply (rule consis_inter_right) apply blast apply blast apply blast apply blast 
-    apply (rule consis_inter_right) apply blast apply blast apply blast apply blast 
-  apply (rule conjI)
-    apply (rule consis_inter_right) apply blast apply blast apply blast apply blast 
-  apply (rule conjI)
-    apply (rule consis_inter_right) apply blast apply blast apply blast apply blast 
-  apply clarify
-  apply (rule conjI)
-    apply (rule consis_inter_right) apply blast apply blast apply blast apply blast 
-    apply (rule consis_inter_right) apply blast apply blast apply blast apply blast 
-  done   
-
-lemma consis_merge_right: "\<lbrakk> v ~ a; v ~ x; wf_ty a; wf_ty x \<rbrakk> \<Longrightarrow> v ~ merge a x"
-  sorry
-
-lemma consis_fold_merge_left: "\<forall> x y. (\<forall> v1 v2. {v1,v2} \<subseteq> set L1 \<longrightarrow> v1 ~ v2) \<longrightarrow>
-        (\<forall> v. v \<in> set L1 \<longrightarrow> x ~ v) \<longrightarrow> (\<forall>v. v \<in> set L1 \<longrightarrow> v ~ y) \<longrightarrow>
-        x ~ y \<longrightarrow> wf_ty x \<longrightarrow> wf_ty y \<longrightarrow>
-       (\<forall>v. v \<in> set L1 \<longrightarrow> wf_ty v)  \<longrightarrow>
-   fold merge L1 x ~ y" (is "\<forall> x y. ?P L1 x y")
-proof (induction L1)
-  case Nil
-  then show ?case by auto
-next
-  case (Cons a L1') then have IH: "\<forall> x y. ?P L1' x y" .
-  show ?case 
-  proof clarify
-    fix x y assume 1: "\<forall>v1 v2. {v1,v2} \<subseteq> set (a # L1') \<longrightarrow> v1 ~ v2" and
-      2: "\<forall>v. v \<in> set (a # L1') \<longrightarrow> x ~ v" and
-      3: "\<forall>v. v \<in> set (a # L1') \<longrightarrow> v ~ y" and
-      x_y: "x ~ y" and wf_x: "wf_ty x" and wf_y: "wf_ty y" and 
-      wf_L1p: "\<forall>v. v \<in> set (a # L1') \<longrightarrow> wf_ty v" 
-    have IH_spec: "?P L1' (merge a x) y" using IH by blast        
-    have wf_a: "wf_ty a" using wf_L1p by auto
-    have "fold merge L1' (merge a x) ~ y"
-    proof (rule IH_spec[rule_format])
-      fix v1 v2 show "{v1, v2} \<subseteq> set L1' \<Longrightarrow> v1 ~ v2" using 1 by auto
-    next fix v assume v_l1: "v \<in> set L1'"
-      have a_v: "a ~ v" using 1 v_l1 by auto
-      have x_v: "x ~ v" using 2 v_l1 by auto
-      show "merge a x ~ v" using consis_merge_left wf_x wf_a a_v x_v by simp
-    next fix v assume "v \<in> set L1'" then show "v ~ y" using 3 by auto
-    next 
-      have a_y: "a ~ y" using 3 by auto
-      show "merge a x ~ y" using a_y x_y wf_a wf_x consis_merge_left by simp
-    next
-      show "wf_ty (merge a x)" using wf_a wf_x by (simp add: "2" consis_sym wf_merge)
-    next show "wf_ty y" using wf_y .
-    next fix v assume "v \<in> set L1'" then show "wf_ty v" using wf_L1p by auto      
-    qed  
-    then show "fold merge (a # L1') x ~ y" by simp
-  qed
-qed
-
-lemma consis_fold_merge_right: "\<forall> x y. (\<forall> v1 v2. {v1,v2} \<subseteq> set L2 \<longrightarrow> v1 ~ v2) \<longrightarrow>
-        (\<forall> v. v \<in> set L2 \<longrightarrow> x ~ v) \<longrightarrow> (\<forall>v. v \<in> set L2 \<longrightarrow> v ~ y) \<longrightarrow>
-        x ~ y \<longrightarrow> wf_ty x \<longrightarrow> wf_ty y \<longrightarrow>
-       (\<forall>v. v \<in> set L2 \<longrightarrow> wf_ty v)  \<longrightarrow>
-   x ~ fold merge L2 y" (is "\<forall> x y. ?P L2 x y")
-  sorry  
-*)
-(*
-lemma consis_fold_merge: "\<forall> L2 x y. (\<forall> v1 v2. {v1,v2} \<subseteq> set L1 \<union> set L2 \<longrightarrow> v1 ~ v2) \<longrightarrow>
-        (\<forall> v. v \<in> set L1 \<union> set L2 \<longrightarrow> x ~ v) \<longrightarrow> (\<forall>v. v \<in> set L1 \<union> set L2 \<longrightarrow> v ~ y) \<longrightarrow>
-        x ~ y \<longrightarrow> wf_ty x \<longrightarrow> wf_ty y \<longrightarrow> 
-       (\<forall>v. v \<in> set L1 \<longrightarrow> wf_ty v) \<and> (\<forall>v. v \<in> set L2 \<longrightarrow> wf_ty v) \<longrightarrow>
-   fold merge L1 x ~ fold merge L2 y" (is "\<forall> L2 x y. ?P L1 L2 x y")
-proof (induction L1)
-  case Nil
-  show ?case
-  proof clarify
-    fix L2 x y assume 1: "\<forall>v1 v2. {v1,v2} \<subseteq> set [] \<union> set L2 \<longrightarrow> v1 ~ v2" and
-      2: "\<forall>v. v \<in> set [] \<union> set L2 \<longrightarrow> x ~ v" and
-      3: "\<forall>v. v \<in> set [] \<union> set L2 \<longrightarrow> v ~ y" and
-      x_y: "x ~ y" and wf_x: "wf_ty x" and wf_y: "wf_ty y" and 
-      wf_L1p: "\<forall>v. v \<in> set [] \<longrightarrow> wf_ty v" and
-      wf_L2: "\<forall>v. v \<in> set L2 \<longrightarrow> wf_ty v"     
-    have "x ~ fold merge L2 y" 
-      apply (rule consis_fold_merge_right[rule_format])
-      using 1 2 3 x_y wf_x wf_y wf_L2 by auto        
-    then show "fold merge [] x ~ fold merge L2 y" by simp
-  qed    
-next
-  case (Cons a L1') then have IH: "\<forall> L2 x y. ?P L1' L2 x y" .
-  show ?case
-  proof clarify
-    fix L2 x y assume 1: "\<forall>v1 v2. {v1,v2} \<subseteq> set (a # L1') \<union> set L2 \<longrightarrow> v1 ~ v2" and
-      2: "\<forall>v. v \<in> set (a # L1') \<union> set L2 \<longrightarrow> x ~ v" and
-      3: "\<forall>v. v \<in> set (a # L1') \<union> set L2 \<longrightarrow> v ~ y" and
-      x_y: "x ~ y" and wf_x: "wf_ty x" and wf_y: "wf_ty y" and 
-      wf_L1p: "\<forall>v. v \<in> set (a # L1') \<longrightarrow> wf_ty v" and
-      wf_L2: "\<forall>v. v \<in> set L2 \<longrightarrow> wf_ty v" 
-    show "fold merge (a # L1') x ~ fold merge L2 y" 
-    proof (cases L2)
-      case Nil
-      show ?thesis 
-        apply (rule consis_fold_merge_left[rule_format])
-          using 1 2 Nil 3 x_y Nil wf_x Nil wf_y wf_L1p by auto
-    next
-      case (Cons b L2')
-      from IH have IH_spec: "?P L1' L2' (merge a x) (merge b y)" by simp        
-      have ax_by: "merge a x ~ merge b y" using 1 2 3 local.Cons x_y consis_merge by auto
-      have 4: "\<forall>v1 v2. {v1,v2} \<subseteq> set L1' \<union> set L2' \<longrightarrow> v1 ~ v2" using 1 Cons by auto
-      have 5: "\<forall>v. v \<in> set L1' \<union> set L2' \<longrightarrow> merge a x ~ v" 
-        apply clarify
-        apply (subgoal_tac "a ~ v") prefer 2 using 1 Cons apply force
-        apply (subgoal_tac "x ~ v") prefer 2 using 2 Cons apply force
-        apply (rule consis_merge_left) apply blast apply blast
-        using wf_L1p apply simp
-        using wf_x apply simp done 
-      have 6: "\<forall>v. v \<in> set L1' \<union> set L2'\<longrightarrow> v ~ merge b y" 
-          apply clarify 
-          apply (subgoal_tac "v ~ b") prefer 2 using 1 Cons apply force
-          apply (subgoal_tac "v ~ y") prefer 2 using 3 Cons apply force
-        apply (rule consis_merge_right) apply blast apply blast
-        using wf_L2 Cons apply simp
-        using wf_y apply simp done 
-      have 8: "wf_ty (merge a x)"
-      proof -
-        have wf_a: "wf_ty a" using wf_L1p by auto
-        have a_x: "a ~ x" using 2 consis_sym[of x a] by simp  
-        show ?thesis using wf_x wf_a a_x wf_merge[of a x] by simp
-      qed
-      have 9: "wf_ty (merge b y)"
-      proof -
-        have wf_b: "wf_ty b" using wf_L2 Cons by auto
-        have b_y: "b ~ y" using 3 consis_sym[of y b] Cons by simp  
-        show ?thesis using wf_y wf_b b_y wf_merge[of b y] by simp
-      qed
-      have 10: "\<forall>v. v \<in> set L1' \<longrightarrow> wf_ty v" using wf_L1p by simp
-      have 11: "\<forall>v. v \<in> set L2' \<longrightarrow> wf_ty v" using wf_L2 Cons by simp
-      have "fold merge L1' (merge a x) ~ fold merge L2' (merge b y)"
-        using IH_spec 4 5 6 8 9 10 11 ax_by by blast          
-      then show ?thesis using Cons by simp
-    qed
-  qed
-qed
-*)
-    
-(*
-lemma consis_merge_list: 
-  assumes c_l12: "\<forall> v1 v2. {v1,v2} \<subseteq> set L1 \<union> set L2 \<longrightarrow> v1 ~ v2" and
-    wf_l1: "\<forall>v. v \<in> set L1 \<longrightarrow> wf_ty v" and
-    wf_l2: "\<forall>v. v \<in> set L2 \<longrightarrow> wf_ty v" and
-    l1_ne: "L1 \<noteq> []" and l2_ne: "L2 \<noteq> []" 
-  shows "\<Prod> L1 ~ \<Prod> L2"
-proof -
-  obtain x L1' where l1: "L1 = x#L1'" using l1_ne by (cases L1) auto
-  obtain y L2' where l2: "L2 = y#L2'" using l2_ne by (cases L2) auto
-  have 1: "\<forall> v1 v2. {v1,v2} \<subseteq> set L1' \<union> set L2' \<longrightarrow> v1 ~ v2" using c_l12 l1 l2 by auto
-  have 2: "\<forall> v. v \<in> set L1' \<union> set L2' \<longrightarrow> x ~ v" using c_l12 l1 l2 by auto
-  have 3: "\<forall>v. v \<in> set L1' \<union> set L2' \<longrightarrow> v ~ y" using c_l12 l1 l2 by auto
-  have 4: "x ~ y" using c_l12 l1 l2 by auto
-  have 5: "wf_ty x" using l1 wf_l1 by auto
-  have 6: "wf_ty y" using l2 wf_l2 by auto
-  have 8: "\<forall>v. v \<in> set L1' \<longrightarrow> wf_ty v" using wf_l1 l1 by auto
-  have 9: "\<forall>v. v \<in> set L2' \<longrightarrow> wf_ty v" using wf_l2 l2 by auto
-  have "fold merge L1' x ~ fold merge L2' y"
-    using consis_fold_merge 1 2 3 4 5 6 8 9 by blast
-  then show ?thesis using l1 l2 merge_list_def by simp
-qed 
-*)
-    
-(*
-lemma d_consis_nat_L: "\<lbrakk> \<Gamma> \<turnstile> c : v; \<Gamma> = [TNat n] \<rbrakk> \<Longrightarrow> v ~ TNat n"
-  apply (induction \<Gamma> c v arbitrary: n rule: deduce_le.induct)
-       apply (case_tac \<Gamma>1) apply force apply force
-      apply (case_tac \<Gamma>1) apply force apply force
-     apply force+
-    apply (case_tac \<Gamma>1) apply force apply force
-   apply force+
-  done
-*)
 
 lemma nat_atoms_consis: "atoms v \<subseteq> {TNat n} \<Longrightarrow> v ~ TNat n"
   by (induction v) auto
@@ -344,19 +153,10 @@ lemma consis_nat_atoms: "\<lbrakk> v ~ TNat n \<rbrakk> \<Longrightarrow> atoms 
   by (induction v arbitrary: n) auto
 
 (*
-  
-(*
-lemma le_any_nat_atom_consis: "\<lbrakk> v \<sqsubseteq> TNat n \<rbrakk> \<Longrightarrow> atoms v \<subseteq> {TNat n}"
-  using le_any_nat_inv_atoms by blast
-*)
 
 definition consis :: "ty set \<Rightarrow> bool" where
   "consis \<Gamma> \<equiv> (\<forall>v v'. v \<in> \<Gamma> \<longrightarrow> v' \<in> \<Gamma> \<longrightarrow> v ~ v')"
   
-*)
-    
-  
-(*   
 lemma val_consis_atoms: "wf_ty v \<Longrightarrow> consis (atoms v)"
   apply (induction v) apply auto
     apply (simp add: consis_def)
@@ -380,36 +180,6 @@ lemma consis_nat_trans2: "\<lbrakk> v1 ~ v2; v2 ~ TNat n \<rbrakk> \<Longrightar
    apply force
   apply force
   done    
-    
-(*
-definition vals :: "ty set \<Rightarrow> bool" where
-  "vals \<Gamma> \<equiv> (\<forall>v. v \<in> \<Gamma> \<longrightarrow> wf_ty v)"
-  
-lemma nat_atom_consis_nat: "\<lbrakk>  TNat n \<in> atoms v; wf_ty v \<rbrakk> \<Longrightarrow> v ~ TNat n"
-  apply (induction v arbitrary: n)
-    apply force
-   apply force
-  apply simp apply clarify apply (erule disjE) 
-   apply (rule conjI) apply force
-    apply (subgoal_tac "v1 ~ TNat n") prefer 2 apply blast 
-  using consis_nat_trans2 consis_sym apply blast
-  apply (rule conjI) 
-   apply (subgoal_tac "v2 ~ TNat n") prefer 2 apply blast
-  using consis_nat_trans2 apply blast
-  apply blast
-  done    
-  
-lemma le_nat_any_consis[intro!]: assumes n_v: "v <: TNat n" and v_v: "wf_ty v" 
-  shows "v ~ TNat n"
-proof -
-  obtain c where "[v] \<turnstile> c : TNat n" using n_v unfolding sub_ty_def by blast
-  then obtain v' where
-    vp_v: "v' \<in> (\<Union>v\<in>set [v]. atoms v)" and vp_n: "v' = TNat n"
-    using d_nat_inv by presburger
-  have "TNat n \<in> atoms v" using vp_v vp_n by simp
-  with v_v show "v ~ TNat n" using nat_atom_consis_nat by blast
-qed    
-*)
  
 lemma consis_inter_right_elim[elim!]: "\<lbrakk> A ~ A1 \<sqinter> A2; \<lbrakk> A ~ A1; A ~ A2 \<rbrakk> \<Longrightarrow> P \<rbrakk> \<Longrightarrow> P"
   using atoms_consis consis_atoms by blast
@@ -428,7 +198,18 @@ lemma meet_list_right_consis_inv: "\<lbrakk> A ~ \<Sqinter>L2; B \<in> set L2; L
 
 lemma meet_list_right_consis: "\<lbrakk> \<forall>B. B \<in> set L2 \<longrightarrow> A ~ B; L2 \<noteq> [] \<rbrakk> \<Longrightarrow> A ~ \<Sqinter>L2"
   using meet_list_atoms atoms_consis consis_atoms by (smt UN_E)
-  
+
+lemma meet_list_singleton[simp]: "\<Sqinter> [a] = a"
+  by (simp add: meet_list_def)
+    
+lemma meet_list_consis: "\<lbrakk> L1 \<noteq> []; L2 \<noteq> []; \<forall>A B. {A,B} \<subseteq> set L1 \<union> set L2 \<longrightarrow> A ~ B\<rbrakk>
+    \<Longrightarrow> \<Sqinter>L1 ~ \<Sqinter>L2"
+ apply (induction L1 arbitrary: L2)
+  apply force
+  apply (case_tac L1)
+    apply simp using meet_list_right_consis apply blast
+  by (simp add: consis_sym meet_list_right_consis)  
+        
 lemma meet_list_left_consis_inv: "\<lbrakk> \<Sqinter>L1 ~ B; A \<in> set L1; L1 \<noteq> [] \<rbrakk> \<Longrightarrow> A ~ B"
   using meet_list_atoms atoms_consis consis_atoms by (smt UN_I)
 
